Rework register allocation for OperandIds
- Adding OperandId and TypedId.
- Adding OperandLocations which are used to determine where an operand
  is stored. Currently on PayloadReg and ValueReg are implemented.
- OperandIds are mapped to OperandLocations using a global Map in
  Boogie.
- Implementing useRegister, useValueRegister, defineRegister and
  defineValueRegister to use operand locations.
- Added OperandId initialization functions that ensure uniquiness and
  initial register allocation to stub inputs.
- Modifying all the stubs to use the new functions.

notes/hacks.bpl
@@ -110,6 +110,394 @@ procedure #MASM~setBigInt($reg: #Reg, $bigInt: #BigInt)
   call #MASM~setValue($reg, tmp'0);
 }
 
+var #CacheIR~knownOperandIds: #Set #OperandId;
+
+var #CacheIR~operandLocations: #Map #OperandId #OperandLocation;
+
+procedure #CacheIR~defineReg($typedId: #TypedId)
+    returns (reg: #Reg)
+    modifies #CacheIR~operandLocations, #CacheIR~allocatedRegs;
+{
+    var $operandId'0: #OperandId;
+    var $loc'0: #OperandLocation;
+    var $loc'1: #OperandLocation;
+    var $locKind'0: #OperandLocationKind;
+    
+    $operandId'0 := #TypedId^to#OperandId($typedId);
+    $loc'0 := #Map~get(#CacheIR~operandLocations, $operandId'0);
+    $locKind'0 := #OperandLocation~kind($loc'0);
+    assert $locKind'0 == #OperandLocationKind^Variant~Uninitialized();
+    
+    call reg := #CacheIR~allocateReg();
+    call $loc'1 := #OperandLocation~setPayloadReg(reg, #TypedId~type($typedId));
+    #CacheIR~operandLocations := #Map~set(#CacheIR~operandLocations, $operandId'0, $loc'1);
+}
+
+procedure #CacheIR~defineValueReg($valueId: #ValueId)
+    returns (reg: #ValueReg)
+    modifies #CacheIR~operandLocations, #CacheIR~allocatedRegs;
+{
+    var $operandId'0: #OperandId;
+    var $loc'0: #OperandLocation;
+    var $loc'1: #OperandLocation;
+    var $locKind'0: #OperandLocationKind;
+    
+    $operandId'0 := #ValueId^to#OperandId($valueId);
+    $loc'0 := #Map~get(#CacheIR~operandLocations, $operandId'0);
+    $locKind'0 := #OperandLocation~kind($loc'0);
+    assert $locKind'0 == #OperandLocationKind^Variant~Uninitialized();
+    
+    call reg := #CacheIR~allocateValueReg();
+    call $loc'1 := #OperandLocation~setValueReg(reg);
+    #CacheIR~operandLocations := #Map~set(#CacheIR~operandLocations, $operandId'0, $loc'1);
+}
+
+procedure #CacheIR~defineObjectReg($id: #ObjectId)
+  returns (ret: #Reg)
+  modifies #CacheIR~operandLocations, #CacheIR~allocatedRegs;
+{
+  var $typedId'v0: #TypedId;
+  var out'0: #TypedId;
+  
+  call out'0 := #TypedId~fromObjectId($id);
+  $typedId'v0 := out'0;
+  call ret := #CacheIR~defineReg($typedId'v0);
+  return;
+}
+
+procedure #CacheIR~defineInt32Reg($id: #Int32Id)
+  returns (ret: #Reg)
+  modifies #CacheIR~operandLocations, #CacheIR~allocatedRegs;
+{
+  var $typedId'v0: #TypedId;
+  var out'0: #TypedId;
+  
+  call out'0 := #TypedId~fromInt32Id($id);
+  $typedId'v0 := out'0;
+  call ret := #CacheIR~defineReg($typedId'v0);
+  return;
+}
+
+procedure #CacheIR~defineNumberReg($id: #NumberId)
+  returns (ret: #ValueReg)
+  modifies #CacheIR~operandLocations, #CacheIR~allocatedRegs;
+{
+  var $valueId'v0: #ValueId;
+  
+  $valueId'v0 := #NumberId^to#ValueId($id);
+  call ret := #CacheIR~defineValueReg($valueId'v0);
+  return;
+}
+
+procedure #CacheIR~defineBooleanReg($id: #BooleanId)
+  returns (ret: #Reg)
+  modifies #CacheIR~operandLocations, #CacheIR~allocatedRegs;
+{
+  var $typedId'v0: #TypedId;
+  var out'0: #TypedId;
+  
+  call out'0 := #TypedId~fromBooleanId($id);
+  $typedId'v0 := out'0;
+  call ret := #CacheIR~defineReg($typedId'v0);
+  return;
+}
+
+procedure #CacheIR~defineStringReg($id: #StringId)
+  returns (ret: #Reg)
+  modifies #CacheIR~operandLocations, #CacheIR~allocatedRegs;
+{
+  var $typedId'v0: #TypedId;
+  var out'0: #TypedId;
+  
+  call out'0 := #TypedId~fromStringId($id);
+  $typedId'v0 := out'0;
+  call ret := #CacheIR~defineReg($typedId'v0);
+  return;
+}
+
+procedure #CacheIR~defineSymbolReg($id: #SymbolId)
+  returns (ret: #Reg)
+  modifies #CacheIR~operandLocations, #CacheIR~allocatedRegs;
+{
+  var $typedId'v0: #TypedId;
+  var out'0: #TypedId;
+  
+  call out'0 := #TypedId~fromSymbolId($id);
+  $typedId'v0 := out'0;
+  call ret := #CacheIR~defineReg($typedId'v0);
+  return;
+}
+
+procedure #CacheIR~defineBigIntReg($id: #BigIntId)
+  returns (ret: #Reg)
+  modifies #CacheIR~operandLocations, #CacheIR~allocatedRegs;
+{
+  var $typedId'v0: #TypedId;
+  var out'0: #TypedId;
+  
+  call out'0 := #TypedId~fromBigIntId($id);
+  $typedId'v0 := out'0;
+  call ret := #CacheIR~defineReg($typedId'v0);
+  return;
+}
+
+procedure #CacheIR~useReg($typedId: #TypedId)
+    returns (reg: #Reg)
+{
+    var $operandId'0: #OperandId;
+    var $loc'0: #OperandLocation;
+    var $locKind'0: #OperandLocationKind;
+    
+    $operandId'0 := #TypedId^to#OperandId($typedId);
+    $loc'0 := #Map~get(#CacheIR~operandLocations, $operandId'0);
+    $locKind'0 := #OperandLocation~kind($loc'0);
+
+    if ($locKind'0 == #OperandLocationKind^Variant~PayloadReg()) {
+        call reg := #OperandLocation~getPayloadReg($loc'0);
+    } else {
+        assert false;
+    }
+}
+
+procedure #CacheIR~useValueReg($valueId: #ValueId)
+    returns (reg: #ValueReg)
+{
+    var $operandId'0: #OperandId;
+    var $loc'0: #OperandLocation;
+    var $locKind'0: #OperandLocationKind;
+    
+    $operandId'0 := #ValueId^to#OperandId($valueId);
+    $loc'0 := #Map~get(#CacheIR~operandLocations, $operandId'0);
+    $locKind'0 := #OperandLocation~kind($loc'0);
+
+    if ($locKind'0 == #OperandLocationKind^Variant~ValueReg()) {
+        call reg := #OperandLocation~getValueReg($loc'0);
+    } else if ($locKind'0 == #OperandLocationKind^Variant~Uninitialized()) { 
+        assert false;
+    } else if ($locKind'0 == #OperandLocationKind^Variant~PayloadReg()) {
+        assert false;
+    } else {
+        assert false;
+    }
+}
+
+procedure #CacheIR~useObjectReg($id: #ObjectId)
+  returns (ret: #Reg)
+{
+  var $typedId'v0: #TypedId;
+  var out'0: #TypedId;
+  
+  call out'0 := #TypedId~fromObjectId($id);
+  $typedId'v0 := out'0;
+  call ret := #CacheIR~useReg($typedId'v0);
+  return;
+}
+
+procedure #CacheIR~useInt32Reg($id: #Int32Id)
+  returns (ret: #Reg)
+{
+  var $typedId'v0: #TypedId;
+  var out'0: #TypedId;
+  
+  call out'0 := #TypedId~fromInt32Id($id);
+  $typedId'v0 := out'0;
+  call ret := #CacheIR~useReg($typedId'v0);
+  return;
+}
+
+procedure #CacheIR~useNumberReg($id: #NumberId)
+  returns (ret: #ValueReg)
+{
+  var $valueId'v0: #ValueId;
+  
+  $valueId'v0 := #NumberId^to#ValueId($id);
+  call ret := #CacheIR~useValueReg($valueId'v0);
+  return;
+}
+
+procedure #CacheIR~useBooleanReg($id: #BooleanId)
+  returns (ret: #Reg)
+{
+  var $typedId'v0: #TypedId;
+  var out'0: #TypedId;
+  
+  call out'0 := #TypedId~fromBooleanId($id);
+  $typedId'v0 := out'0;
+  call ret := #CacheIR~useReg($typedId'v0);
+  return;
+}
+
+procedure #CacheIR~useStringReg($id: #StringId)
+  returns (ret: #Reg)
+{
+  var $typedId'v0: #TypedId;
+  var out'0: #TypedId;
+  
+  call out'0 := #TypedId~fromStringId($id);
+  $typedId'v0 := out'0;
+  call ret := #CacheIR~useReg($typedId'v0);
+  return;
+}
+
+procedure #CacheIR~useSymbolReg($id: #SymbolId)
+  returns (ret: #Reg)
+{
+  var $typedId'v0: #TypedId;
+  var out'0: #TypedId;
+  
+  call out'0 := #TypedId~fromSymbolId($id);
+  $typedId'v0 := out'0;
+  call ret := #CacheIR~useReg($typedId'v0);
+  return;
+}
+
+procedure #CacheIR~useBigIntReg($id: #BigIntId)
+  returns (ret: #Reg)
+{
+  var $typedId'v0: #TypedId;
+  var out'0: #TypedId;
+  
+  call out'0 := #TypedId~fromBigIntId($id);
+  $typedId'v0 := out'0;
+  call ret := #CacheIR~useReg($typedId'v0);
+  return;
+}
+
+procedure #CacheIR~initInputLocation($typedId: #TypedId)
+    modifies #CacheIR~operandLocations;
+{
+    var $operandId'0: #OperandId;
+    var tmp'0: #Bool;
+    var $loc'0: #OperandLocation;
+
+    $operandId'0 := #TypedId^to#OperandId($typedId);
+    call $loc'0 := #OperandLocation~newUninitialized();
+    tmp'0 := #Set~contains(#CacheIR~knownOperandIds, $operandId'0);
+    assume !tmp'0;
+    #CacheIR~knownOperandIds := #Set~add(#CacheIR~knownOperandIds, $operandId'0);
+    #CacheIR~operandLocations := #Map~set(#CacheIR~operandLocations, $operandId'0, $loc'0);
+}
+
+procedure #CacheIR~initValueInputLocation($valueId: #ValueId)
+    modifies #CacheIR~operandLocations;
+{
+    var $operandId'0: #OperandId;
+    var tmp'0: #Bool;
+    var $loc'0: #OperandLocation;
+
+    $operandId'0 := #ValueId^to#OperandId($valueId);
+    tmp'0 := #Set~contains(#CacheIR~knownOperandIds, $operandId'0);
+    assume !tmp'0;
+    #CacheIR~knownOperandIds := #Set~add(#CacheIR~knownOperandIds, $operandId'0);
+
+    call $loc'0 := #OperandLocation~newUninitialized();
+    #CacheIR~operandLocations := #Map~set(#CacheIR~operandLocations, $operandId'0, $loc'0);
+}
+
+procedure #CacheIR~initInput($typedId: #TypedId)
+    modifies #CacheIR~operandLocations, #CacheIR~allocatedRegs;
+{
+  var out'0: #Reg;
+  
+  call #CacheIR~initInputLocation($typedId);
+  call out'0 := #CacheIR~defineReg($typedId);
+  return;
+}
+
+procedure #CacheIR~initValueInput($valueId: #ValueId)
+    modifies #CacheIR~operandLocations, #CacheIR~allocatedRegs;
+{
+  var out'0: #ValueReg;
+  
+  call #CacheIR~initValueInputLocation($valueId);
+  call out'0 := #CacheIR~defineValueReg($valueId);
+  return;
+}
+
+procedure #CacheIR~initObjectInput($id: #ObjectId)
+    modifies #CacheIR~operandLocations, #CacheIR~allocatedRegs;
+{
+  var $typedId'v0: #TypedId;
+  var out'0: #TypedId;
+  
+  call out'0 := #TypedId~fromObjectId($id);
+  $typedId'v0 := out'0;
+  call #CacheIR~initInput($typedId'v0);
+  return;
+}
+
+procedure #CacheIR~initInt32Input($id: #Int32Id)
+    modifies #CacheIR~operandLocations, #CacheIR~allocatedRegs;
+{
+  var $typedId'v0: #TypedId;
+  var out'0: #TypedId;
+  
+  call out'0 := #TypedId~fromInt32Id($id);
+  $typedId'v0 := out'0;
+  call #CacheIR~initInput($typedId'v0);
+  return;
+}
+
+procedure #CacheIR~initNumberInput($id: #NumberId)
+    modifies #CacheIR~operandLocations, #CacheIR~allocatedRegs;
+{
+  var $valueId'v0: #ValueId;
+  
+  $valueId'v0 := #NumberId^to#ValueId($id);
+  call #CacheIR~initValueInput($valueId'v0);
+  return;
+}
+
+procedure #CacheIR~initBooleanInput($id: #BooleanId)
+    modifies #CacheIR~operandLocations, #CacheIR~allocatedRegs;
+{
+  var $typedId'v0: #TypedId;
+  var out'0: #TypedId;
+  
+  call out'0 := #TypedId~fromBooleanId($id);
+  $typedId'v0 := out'0;
+  call #CacheIR~initInput($typedId'v0);
+  return;
+}
+
+procedure #CacheIR~initStringInput($id: #StringId)
+    modifies #CacheIR~operandLocations, #CacheIR~allocatedRegs;
+{
+  var $typedId'v0: #TypedId;
+  var out'0: #TypedId;
+  
+  call out'0 := #TypedId~fromStringId($id);
+  $typedId'v0 := out'0;
+  call #CacheIR~initInput($typedId'v0);
+  return;
+}
+
+procedure #CacheIR~initSymbolInput($id: #SymbolId)
+    modifies #CacheIR~operandLocations, #CacheIR~allocatedRegs;
+{
+  var $typedId'v0: #TypedId;
+  var out'0: #TypedId;
+  
+  call out'0 := #TypedId~fromSymbolId($id);
+  $typedId'v0 := out'0;
+  call #CacheIR~initInput($typedId'v0);
+  return;
+}
+
+procedure #CacheIR~initBigIntInput($id: #BigIntId)
+    modifies #CacheIR~operandLocations, #CacheIR~allocatedRegs;
+{
+  var $typedId'v0: #TypedId;
+  var out'0: #TypedId;
+  
+  call out'0 := #TypedId~fromBigIntId($id);
+  $typedId'v0 := out'0;
+  call #CacheIR~initInput($typedId'v0);
+  return;
+}
+
+var #CacheIR~allocatedRegs: #Set #Reg;
+
 procedure #CacheIR~allocateValueReg()
   returns (ret: #ValueReg)
   modifies #CacheIR~allocatedRegs;
@@ -122,8 +510,6 @@ procedure #CacheIR~releaseValueReg($valueReg: #ValueReg)
 {
   call #CacheIR~releaseReg($valueReg);
 }
-
-var #CacheIR~allocatedRegs: #Set #Reg;
 
 procedure #CacheIR~allocateReg()
   returns (ret: #Reg)
